src/Narcissus/BinLib.v
@@ -13,6 +13,44 @@ Require Export
 
 Global Instance ByteStringQueueMonoid : Monoid ByteString := ByteStringQueueMonoid.
 
+(* Here are the expected correctness lemmas for optimized versions of the synthesized functions. *)
+Lemma CorrectDecodeEncode
+      {A} {cache : Cache.Cache}
+      {sz}
+  : forall Invariant
+           (FormatSpec : Specs.FormatM A _)
+           (encoder : CorrectAlignedEncoderFor FormatSpec Invariant)
+           (decoder : CorrectAlignedDecoderFor Invariant FormatSpec),
+    forall a ce cd v,
+      Cache.Equiv ce cd
+      -> Invariant a
+      -> snd (projT1 (projT2 decoder)) cd
+      -> forall cd' idx ce' v',
+          projT1 encoder a sz v 0 ce = Some (v', idx, ce')
+          -> (projT1 decoder sz) v' 0 cd = Some (a, idx, cd').
+Proof.
+  intros.
+  destruct encoder as [aligned_encoder aligned_encoder_OK].
+  simpl in *; specialize (aligned_encoder_OK _ H0).
+  destruct aligned_encoder_OK as [encoder [encoder_OK [padding_OK encoder_equiv] ] ].
+  destruct decoder as [aligned_decoder [ [decoder Inv] [ [Inv' [decoder_OK Inv_cd] ] decoder_equiv ] ] ]; simpl in *.
+  specialize (decoder_OK Inv_cd).
+Abort.
+(* specialize (encoder_OK ce _ (Core.ReturnComputes _)) .
+  destruct (encoder_equiv ce 0) as [? [? ?] ].
+  specialize (H3 (padding_OK _)).
+
+  destruct decoder_equiv.
+
+  specialize (encoder_OK a ce _ (ReturnComputes _)) .
+  destruct decoder_OK as [decoder_OK _].
+  destruct (encoder a ce) as [bin ce'].
+  unfold cache_inv_Property in Inv_cd.
+  eapply decoder_OK  with (ext := mempty) in encoder_OK; eauto.
+  destruct_ex; intuition.
+  rewrite mempty_right in H3; eauto.
+Qed. *)
+
 (* Various Constants that clients should never simplify. *)
 Global Arguments split1 : simpl never.
 Global Arguments split2 : simpl never.
